Suspicious progress on LRU cache

Test/tutorial/LRU_cache/two.dfy
@@ -8,14 +8,33 @@ trait Storage<T(!new)> {
 
 	ghost var log: seq<entry<T>>
 
+	function last_occurence_pre(key: nat, log': seq<entry<T>>): Outcome<T> {
+		var size: nat := |log'|;
+		if size == 0 then
+			Failure
+		else
+			var candidate: entry := log'[size-1];
+			if candidate.key == key then
+				Success(candidate.value)
+			else
+				last_occurence_pre(key, log'[..(size-1)])
+	}
+
+	function last_occurence(key: nat): Outcome<T>
+		reads this
+	{
+		last_occurence_pre(key,log)
+	}
+	
 	predicate Invariant()
 		reads this
 
 	method get(key: nat) returns (result: Outcome<T>)
 		requires Invariant()
 		ensures Invariant()
-		ensures result.Success? <==> exists index: nat :: index < |log| && log[index].key == key
+		ensures result.Success? <==> exists index: nat :: index < |log| && log[index].key == key 
 		ensures result.Failure? <==> !exists index: nat :: index < |log| && log[index].key == key
+		ensures result.Success? ==> last_occurence(key).Success? && last_occurence(key).value == result.value
 		
 	function method fget(key: nat): Outcome<T>
  		reads this
@@ -32,11 +51,12 @@ trait Storage<T(!new)> {
 class MapStorage<T(!new)> extends Storage<T> {
 
 	var storage: map<nat,T>
-
+		
 	predicate Invariant()
 		reads this
 	{
-		&& forall key: nat :: key in storage <==> exists index: nat :: index < |log| && log[index].key == key
+		&& (forall key: nat :: key in storage <==> exists index: nat :: index < |log| && log[index].key == key)
+		&& (forall key: nat :: forall value: T :: (key in storage && storage[key] == value) ==> last_occurence(key).Success? && last_occurence(key).value == value)
 	}
 	
 	constructor()
@@ -51,6 +71,7 @@ class MapStorage<T(!new)> extends Storage<T> {
 		ensures Invariant()
 		ensures result.Success? <==> exists index: nat :: index < |log| && log[index].key == key
 		ensures result.Failure? <==> !exists index: nat :: index < |log| && log[index].key == key
+		ensures result.Success? ==> last_occurence(key).Success? && last_occurence(key).value == result.value
 	{
 		if key in storage {
 			result := Success(storage[key]);
